bool/btauto.ml4
@@ -1,0 +1,175 @@
+let contrib_name = "btauto"
+
+let init_constant dir s =
+  let find_constant contrib dir s =
+    Libnames.constr_of_global (Coqlib.find_reference contrib dir s)
+  in
+  find_constant contrib_name dir s
+
+let get_constant dir s = lazy (init_constant dir s)
+
+let decomp_term (c : Term.constr)  = 
+  Term.kind_of_term (Term.strip_outer_cast c)
+    
+let lapp c v  = Term.mkApp (Lazy.force c, v)
+
+let (===) = Term.eq_constr
+
+module CoqList = struct
+  let path = ["Coq"; "Init"; "Datatypes"]
+  let typ = get_constant path "list"
+  let nil = get_constant path "nil"
+  let cons = get_constant path "cons"
+
+  let cons ty h t = lapp cons [|ty; h ; t|]
+  let nil ty = lapp nil [|ty|]
+  let rec of_list ty = function
+    | [] -> nil ty
+    | t::q -> cons ty t (of_list ty q)
+  let type_of_list ty = lapp typ [|ty|]
+
+end
+
+module CoqNat = struct
+  let path = ["Coq"; "Init"; "Datatypes"]
+  let typ = get_constant path "nat"
+  let _S = get_constant path "S"
+  let _O = get_constant path "O"
+
+  (* A coq nat from an int *)
+  let rec of_int n =
+    if n <= 0 then Lazy.force _O
+    else
+      let ans = of_int (pred n) in
+      lapp _S [|ans|]
+
+end
+
+module Env = struct
+
+  module ConstrHashed = struct
+    type t = Term.constr
+    let equal = Term.eq_constr
+    let hash = Term.hash_constr
+  end
+
+  module ConstrHashtbl = Hashtbl.Make (ConstrHashed)
+
+  type t = (int ConstrHashtbl.t * int ref)
+      
+  let add (tbl, off) (t : Term.constr) =
+    try ConstrHashtbl.find tbl t 
+    with
+    | Not_found -> 
+      let i = !off in 
+      let () = ConstrHashtbl.add tbl t i in
+      let () = incr off in
+      i
+
+  let empty () = (ConstrHashtbl.create 16, ref 0)       
+
+  let to_list (env, _) = 
+    ConstrHashtbl.fold (fun constr key acc -> constr :: acc) env []
+      
+end
+
+module Bool = struct
+
+  let typ = get_constant ["Coq"; "Init"; "Datatypes"] "bool"
+  let trueb = get_constant ["Coq"; "Init"; "Datatypes"] "true"
+  let falseb = get_constant ["Coq"; "Init"; "Datatypes"] "false"
+  let andb = get_constant ["Coq"; "Init"; "Datatypes"] "andb"
+  let orb = get_constant ["Coq"; "Init"; "Datatypes"] "orb"
+  let xorb = get_constant ["Coq"; "Init"; "Datatypes"] "xorb"
+  let negb = get_constant ["Coq"; "Init"; "Datatypes"] "negb"
+
+  type t =
+  | Var of int
+  | Const of bool
+  | Andb of t * t
+  | Orb of t * t
+  | Xorb of t * t
+  | Negb of t
+  | Ifb of t * t * t
+
+  let quote (env : Env.t) (c : Term.constr) : t =
+    let trueb = Lazy.force trueb in
+    let falseb = Lazy.force falseb in
+    let andb = Lazy.force andb in
+    let orb = Lazy.force orb in
+    let xorb = Lazy.force xorb in
+    let negb = Lazy.force negb in
+
+    let rec aux c = match decomp_term c with
+    | Term.App (head, args) ->
+      if head === andb && Array.length args = 2 then
+        Andb (aux args.(0), aux args.(1))
+      else if head === orb && Array.length args = 2 then
+        Orb (aux args.(0), aux args.(1))
+      else if head === xorb && Array.length args = 2 then
+        Xorb (aux args.(0), aux args.(1))
+      else if head === negb && Array.length args = 1 then
+        Negb (aux args.(0))
+      else Var (Env.add env c)
+    | _ ->
+      if c === falseb then Const false
+      else if c === trueb then Const true
+      else Var (Env.add env c)
+    in
+    aux c
+
+end
+
+module Btauto = struct
+
+  let f_var = get_constant ["Btauto"; "Reflect"] "formula_var"
+  let f_btm = get_constant ["Btauto"; "Reflect"] "formula_btm"
+  let f_top = get_constant ["Btauto"; "Reflect"] "formula_top"
+  let f_cnj = get_constant ["Btauto"; "Reflect"] "formula_cnj"
+  let f_dsj = get_constant ["Btauto"; "Reflect"] "formula_dsj"
+  let f_neg = get_constant ["Btauto"; "Reflect"] "formula_neg"
+
+  let eval = get_constant ["Btauto"; "Reflect"] "formula_eval"
+
+  let rec convert = function
+  | Bool.Var n -> lapp f_var [|CoqNat.of_int n|]
+  | Bool.Const true -> Lazy.force f_top
+  | Bool.Const false -> Lazy.force f_btm
+  | Bool.Andb (b1, b2) -> lapp f_cnj [|convert b1; convert b2|]
+  | Bool.Orb (b1, b2) -> lapp f_dsj [|convert b1; convert b2|]
+  | Bool.Negb b -> lapp f_neg [|convert b|]
+  | _ -> assert false
+
+  let convert_env env : Term.constr = 
+    let l = Env.to_list env in 
+    CoqList.of_list (Lazy.force Bool.typ) l
+
+  let reify env t = lapp eval [|convert_env env; convert t|]
+
+  let tac gl =
+    Tactics.change_in_concl None (Lazy.force Bool.trueb) gl
+
+  let tac gl =
+    let concl = Tacmach.pf_concl gl in
+    let t = decomp_term concl in
+    match t with
+    | Term.App (c, args) when Array.length args >= 2 ->
+      let len = Array.length args in
+      let tl = args.(len - 2) in
+      let tr = args.(len - 1) in
+      let ts = Array.sub args 0 (len - 2) in
+      let rel = Term.mkApp (c, ts) in
+      let env = Env.empty () in
+      let fl = Bool.quote env tl in
+      let fr = Bool.quote env tr in
+      let changed_gl = Term.mkApp (rel, [|reify env fl; reify env fr|]) in
+      Tactics.change_in_concl None changed_gl gl
+    | _ ->
+      let msg = Pp.str "Cannot recognize a boolean equality" in
+      Tacticals.tclFAIL 1 msg gl
+
+end
+
+TACTIC EXTEND _btauto_
+| [ "btauto" ] -> [ Btauto.tac ]
+END
